Drop let for now

SimplyTypedLambdaCalculus.thy
@@ -6,6 +6,8 @@ begin
 
 type_synonym var = string
 
+no_notation Set.member ("(_/ \<in> _)" [51, 51] 50)
+
 datatype type = TUnit
   | TApp type type ("_ \<rightarrow> _")
 
@@ -14,36 +16,37 @@ datatype expr =
   | Var var
   | Abs var type expr
   | App expr expr
-  | Let var expr expr
 
-type_synonym ctx = "(var \<times> type) set"
+(* it is important to choose a list here, since this defines how the type lookup is made
+   when augmenting the context *)
+type_synonym ctx = "(var \<times> type) list"
+
+fun has_type_in_ctx :: "var \<times> type \<Rightarrow> ctx \<Rightarrow> bool" ("(_ \<in> _)" [51, 51] 50) where
+  "has_type_in_ctx    _          [] = False" |
+  "has_type_in_ctx (x,\<tau>) ((y,\<tau>')#\<Gamma>) = (if x = y then \<tau> = \<tau>' else has_type_in_ctx (x,\<tau>) \<Gamma>)"
 
 inductive "value" :: "expr \<Rightarrow> bool" where
-  Unit: "value Unit"
-| Fn: "value (Abs x t e1)"
+  ValueUnit: "value Unit"
+| ValueFn: "value (Abs x t e1)"
 
 declare value.intros[simp,intro]
 
 fun fvs :: "expr \<Rightarrow> var set" where
   "fvs Unit          = {}" |
   "fvs (Var v)       = {v}" |
-  "fvs (Abs v ty e)  = fvs e - {v}" |
-  "fvs (App e1 e2)   = fvs e1 \<union> fvs e2" |
-  "fvs (Let x e1 e2) = (fvs e1 \<union> fvs e2) - {x}"
+  "fvs (Abs x ty e)  = fvs e - {x}" |
+  "fvs (App e1 e2)   = fvs e1 \<union> fvs e2"
 
 fun subst :: "var \<Rightarrow> expr \<Rightarrow> expr \<Rightarrow> expr" where
   "subst x t Unit         = Unit" |
   "subst x t (Var v)      = (if x = v then t else Var v)" |
   "subst x t (Abs v ty e) = Abs v ty (if x = v then e else subst x t e)" |
-  "subst x t (App e1 e2)  = App (subst x t e1) (subst x t e2)" |
-  "subst x t (Let v t' e) = Let v (if x = v then t' else subst x t t') (if x = v then e else subst x t e)"
+  "subst x t (App e1 e2)  = App (subst x t e1) (subst x t e2)"
 
 inductive reduce :: "expr \<Rightarrow> expr \<Rightarrow> bool" where
   CApp1: "reduce e1 e1' \<Longrightarrow> reduce (App e1 e2) (App e1' e2)"
 | CApp2: "value e1      \<Longrightarrow> reduce e2 e2' \<Longrightarrow> reduce (App e1 e2) (App e1 e2')"
 | RApp:  "value e2      \<Longrightarrow> reduce (App (Abs x ty e1) e2) (subst x e2 e1)"
-| CLet:  "reduce e1 e1' \<Longrightarrow> reduce (Let x e1 e2) (Let x e1' e2)"
-| RLet:  "value e1      \<Longrightarrow> reduce (Let x e1 e2) (subst x e1 e2)"
 
 declare reduce.intros[simp,intro]
 
@@ -53,9 +56,8 @@ inductive_cases ReduceElimE[elim]: "reduce (Let x e1 e2) e"
 inductive has_type :: "ctx \<Rightarrow> expr \<Rightarrow> type \<Rightarrow> bool" ("_ \<turnstile> _ : _" [40,40,40]) where
   TypeUnit: "\<Gamma> \<turnstile> Unit : TUnit" |
   TypeVar:  "(x, \<tau>) \<in> \<Gamma> \<Longrightarrow> \<Gamma> \<turnstile> (Var x) : \<tau>" |
-  TypeFn:   "\<lbrakk> (insert (x, \<tau>) \<Gamma>) \<turnstile> e : \<tau>' \<rbrakk> \<Longrightarrow> \<Gamma> \<turnstile> (Abs x \<tau> e) : (\<tau> \<rightarrow> \<tau>')" |
-  TypeApp:  "\<lbrakk> \<Gamma> \<turnstile> e1 : (\<tau>' \<rightarrow> \<tau>); \<Gamma> \<turnstile> e2 : \<tau>' \<rbrakk> \<Longrightarrow> \<Gamma> \<turnstile> (App e1 e2) : \<tau>" |
-  TypeLet:  "\<lbrakk> \<Gamma> \<turnstile> e1 : \<tau>\<^sub>1; (insert (x, \<tau>\<^sub>1) \<Gamma>) \<turnstile> e2 : \<tau>\<^sub>2 \<rbrakk> \<Longrightarrow> \<Gamma> \<turnstile> (Let x e1 e2) : \<tau>\<^sub>2"
+  TypeFn:   "\<lbrakk> ((x, \<tau>)#\<Gamma>) \<turnstile> e : \<tau>' \<rbrakk> \<Longrightarrow> \<Gamma> \<turnstile> (Abs x \<tau> e) : (\<tau> \<rightarrow> \<tau>')" |
+  TypeApp:  "\<lbrakk> \<Gamma> \<turnstile> e1 : (\<tau>' \<rightarrow> \<tau>); \<Gamma> \<turnstile> e2 : \<tau>' \<rbrakk> \<Longrightarrow> \<Gamma> \<turnstile> (App e1 e2) : \<tau>"
 
 declare has_type.intros[simp,intro]
 
@@ -63,7 +65,6 @@ inductive_cases TypeUnitE[elim!]: "\<Gamma> \<turnstile> Unit : \<tau>"
 inductive_cases TypeVarE[elim!]:  "\<Gamma> \<turnstile> (Var x) : \<tau>"
 inductive_cases TypeFnE[elim]:    "\<Gamma> \<turnstile> (Abs x \<tau> e) : \<tau>"
 inductive_cases TypeAppE[elim]:   "\<Gamma> \<turnstile> (App e1 e2) : \<tau>"
-inductive_cases TypeLet[elim]:    "\<Gamma> \<turnstile> (Let x e1 e2) : \<tau>"
 
 inductive step_or_value where
   IsValue: "value e \<Longrightarrow> step_or_value e" |
@@ -83,29 +84,65 @@ lemma identity_exists:
   by (metis RApp subst.simps(2))
 
 theorem progress:
-  "{} \<turnstile> e : \<tau> \<Longrightarrow> step_or_value e"
-proof (induction  "{} :: (var \<times> type) set" "e" "\<tau>" rule:has_type.induct)
+  "[] \<turnstile> e : \<tau> \<Longrightarrow> step_or_value e"
+proof (induction  "[] :: ctx" "e" "\<tau>" rule:has_type.induct)
   case (TypeApp e1 \<tau>' \<tau> e2)
   then show ?case
     (* found by sledgehammer *)
-    by (metis CApp1 CApp2 IsStep RApp StepOrValueE TypeUnitE type.distinct(1) value.simps)
-qed blast+
+    using step_or_value.simps value.simps by auto
+qed auto
+
+lemma context_strengthening:
+  "\<Gamma> \<turnstile> e : \<tau> \<Longrightarrow> \<forall>x \<tau>'. Set.member x (fvs e) \<longrightarrow> (x, \<tau>') \<in> \<Gamma> \<longrightarrow> (x, \<tau>') \<in> \<Gamma>' \<Longrightarrow> \<Gamma>' \<turnstile> e : \<tau>"
+proof (induction arbitrary: \<Gamma>' rule: has_type.induct)
+  case (TypeApp \<Gamma> e1 \<tau>' \<tau> e2)
+  then show ?case
+    (* found by sledgehammer *)
+    by (metis Un_iff fvs.simps(4) has_type.TypeApp)
+qed auto
+
+lemma well_typed_fvs:
+  "\<Gamma> \<turnstile> e : \<tau> \<Longrightarrow> \<forall>v \<in> fvs e. (\<exists>\<tau>. (v, \<tau>) \<in> \<Gamma>)"
+  apply (induction rule:has_type.induct, auto)
+  by metis+
+
+corollary well_typed_no_fvs:
+  "[] \<turnstile> e : \<tau> \<Longrightarrow> fvs e = {}"
+  (* sledgehammer *)
+  by (meson ex_in_conv has_type_in_ctx.simps(1) well_typed_fvs)
 
 lemma subst_preservation:
-  "(insert (x, \<tau>') \<Gamma>) \<turnstile> e2 : \<tau> \<Longrightarrow> {} \<turnstile> e1 : \<tau>' \<Longrightarrow> \<Gamma> \<turnstile> subst x e1 e2 : \<tau>"
-  sorry
+  "\<lbrakk> ((x, \<tau>')#\<Gamma>) \<turnstile> e2 : \<tau>; [] \<turnstile> e1 : \<tau>' \<rbrakk>
+   \<Longrightarrow> \<Gamma> \<turnstile> subst x e1 e2 : \<tau>"
+proof (induct e2 arbitrary: \<Gamma> \<tau> \<tau>' x)
+  case (Var v)
+  then show ?case
+    (* found by sledgehammer *)
+    by (metis TypeVar TypeVarE context_strengthening has_type_in_ctx.simps(1) has_type_in_ctx.simps(2) subst.simps(2))
+next
+  case (Abs y \<sigma> e)
+  then show ?case
+  proof (cases "x = y")
+    case False
+    with Abs(2) obtain \<tau>\<^sub>2 where "\<tau> = (\<sigma> \<rightarrow> \<tau>\<^sub>2)" "((y, \<sigma>)#(x, \<tau>')#\<Gamma>) \<turnstile> e : \<tau>\<^sub>2"
+      by (induct "(x, \<tau>') # \<Gamma>" "Abs y \<sigma> e" "\<tau>" rule:has_type.induct, blast)
+    then have "((x, \<tau>')#(y, \<sigma>)#\<Gamma>) \<turnstile> e : \<tau>\<^sub>2"
+      (* found by sledgehammer *)
+      using False context_strengthening has_type_in_ctx.simps(2) by presburger
+    then show ?thesis
+      (* found by sledgehammer *)
+      by (simp add: Abs.hyps Abs.prems(2) False \<open>\<tau> = \<sigma> \<rightarrow> \<tau>\<^sub>2\<close>)
+  qed (auto simp: context_strengthening)
+qed fastforce+
 
 theorem preservation:
-  "reduce e e' \<Longrightarrow> {} \<turnstile> e : \<tau> \<Longrightarrow> {} \<turnstile> e' : \<tau>"
+  "reduce e e' \<Longrightarrow> [] \<turnstile> e : \<tau> \<Longrightarrow> [] \<turnstile> e' : \<tau>"
 proof (induct arbitrary: \<tau> rule:reduce.induct)
   case (RApp e2 x \<tau>' e)
-  from RApp.prems RApp.hyps show ?case
-    by (induct "{} :: ctx" "App (Abs x \<tau>' e) e2" "\<tau>")
-       (metis TypeFnE TypeVar dual_order.refl insert_subset subst.simps(2) subst_preservation)
-next
-  case (RLet e1 x e2)
-  then show ?case
-    by (auto simp: subst_preservation)
+  from RApp.prems show ?case
+    by (induct "[] :: ctx" "App (Abs x \<tau>' e) e2" "\<tau>")
+       (* found by sledgehammer *)
+       (metis expr.inject(2) expr.simps(11) expr.simps(15) expr.simps(7) has_type.simps subst_preservation type.inject)
 qed blast+
 
 
